skeleton of proof is now repaired - some holes remain for now

sha/verif_hmacNK_init_part2.v
@@ -14,7 +14,7 @@ Require Import hmac_pure_lemmas.
 Require Import hmac_common_lemmas.
 
 Require Import sha.hmac_NK.
-Require Import sha.verif_hmacNK_init_part1.
+Require Import sha.verif_hmacNK_init_part1. (*part1 now takes 1h to compile*)
 
 Lemma isbyte_zeroExt8: forall x, isbyteZ x -> Int.repr x = (Int.zero_ext 8 (Int.repr x)).
 Proof. intros. rewrite zero_ext_inrange. trivial.
@@ -69,24 +69,7 @@ Proof. intros. apply Znth_map_Vint_is_int_I8.
   rewrite Zlength_map; trivial.
 Qed.
 
-Definition FIRSTN {A} i (l:list A) := firstn (Z.to_nat i) l.
-
-Lemma FIRSTN_precise {A} n (l:list A) (H: Zlength l = n): FIRSTN n l = l.
-Proof. unfold FIRSTN.
-       apply firstn_precise. subst n. apply Zlength_length; trivial. apply Zlength_nonneg.
-Qed.
-
-Lemma FIRSTN_zero {A} (l:list A): FIRSTN 0 l = []. Proof. reflexivity. Qed.
-
-Definition SKIPN {A} i (l:list A) := skipn (Z.to_nat i) l.
-
-Lemma SKIPn_short {A : Type} n (al : list A): (Zlength al <= n) -> SKIPN n al = [].
-Proof. unfold SKIPN. intros. apply skipn_short. 
-       rewrite Zlength_correct in H. rewrite <- (Nat2Z.id (length al)). 
-       rewrite (Z2Nat.inj_le _ n) in H. omega. specialize (Zlength_nonneg al); rewrite Zlength_correct. trivial.
-       specialize (Zlength_nonneg al); rewrite Zlength_correct. intros; omega. 
-Qed.
-
+(*
 Lemma UPD_IPAD: forall
   (key : list Z)
   (ZLI : Zlength
@@ -250,9 +233,12 @@ Proof. intros.
               do 2 rewrite map_length. unfold HMAC_SHA256.mkArgZ in ZLO'; rewrite ZLO'.
                        apply Z2Nat.inj_le; omega.
 Qed.
-
+*)
+Check t_struct_SHA256state_st. 
+(*Definition postResetHMS (iS oS: s256state): hmacstate :=
+  (emptySha, (iS, oS)).*)
 Definition postResetHMS (iS oS: s256state): hmacstate :=
-  (emptySha, (iS, oS)).
+  (default_val t_struct_SHA256state_st, (iS, oS)).
 
 Definition initPostResetConditional r (c:val) (k: val) h key iS oS: mpred:=
   match k with
@@ -265,6 +251,304 @@ Definition initPostResetConditional r (c:val) (k: val) h key iS oS: mpred:=
                         (data_at Tsh (tarray tuchar (Zlength key)) (map Vint (map Int.repr key)) (Vptr b ofs)))
   | _ => FF
   end.
+
+Lemma ipad_loop Espec pb pofs cb cofs ckb ckoff kb kofs l key kv
+(HMS' : reptype t_struct_hmac_ctx_st) (FR:mpred): forall
+(KL1 : l = Zlength key)
+(KL2 : 0 <= l <= Int.max_signed)
+(KL3 : l * 8 < two_p 64)
+(KHMS : HMS' = HMS)
+(IPADcont : list val)
+(HeqIPADcont : IPADcont =
+              map Vint
+                (map Int.repr
+                   (map Byte.unsigned
+                      (HMAC_SHA256.mkArg
+                         (map Byte.repr (HMAC_SHA256.mkKey key)) Ipad))))
+(ZLI : Zlength
+        (HMAC_SHA256.mkArgZ (map Byte.repr (HMAC_SHA256.mkKey key)) Ipad) =
+      64)
+(isbyte_key : Forall isbyteZ key),
+@semax CompSpecs Espec
+  (initialized _reset (func_tycontext f_HMAC_Init HmacVarSpecs HmacFunSpecs))
+  (PROP  ()
+   LOCAL  (temp _reset (Vint (Int.repr 1));
+   lvar _ctx_key (Tarray tuchar 64 noattr) (Vptr ckb ckoff);
+   lvar _pad (Tarray tuchar 64 noattr) (Vptr pb pofs);
+   temp _ctx (Vptr cb cofs); temp _key (Vptr kb kofs);
+   temp _len (Vint (Int.repr l)); gvar sha._K256 kv)
+   SEP  ( (*`(K_vector kv);*) `(FR);
+   `(data_at Tsh (Tarray tuchar 64 noattr)
+       (default_val (Tarray tuchar 64 noattr)) (Vptr pb pofs));
+   (*`(data_at Tsh t_struct_hmac_ctx_st HMS' (Vptr cb cofs));*)
+   `(data_at Tsh (tarray tuchar 64)
+       (map Vint (map Int.repr (HMAC_SHA256.mkKey key))) (Vptr ckb ckoff)) (*;
+   `(data_at Tsh (tarray tuchar (Zlength key)) (map Vint (map Int.repr key))
+       (Vptr kb kofs))*)))
+  (Sfor (Sset _i (Econst_int (Int.repr 0) tint))
+     (Ebinop Olt (Etempvar _i tint) (Econst_int (Int.repr 64) tint) tint)
+     (Ssequence
+        (Sset _aux
+           (Ecast
+              (Ederef
+                 (Ebinop Oadd (Evar _ctx_key (Tarray tuchar 64 noattr))
+                    (Etempvar _i tint) (tptr tuchar)) tuchar) tuchar))
+        (Ssequence
+           (Sset _aux
+              (Ecast
+                 (Ebinop Oxor (Econst_int (Int.repr 54) tint)
+                    (Etempvar _aux tuchar) tint) tuchar))
+           (Sassign
+              (Ederef
+                 (Ebinop Oadd (Evar _pad (Tarray tuchar 64 noattr))
+                    (Etempvar _i tint) (tptr tuchar)) tuchar)
+              (Etempvar _aux tuchar))))
+     (Sset _i
+        (Ebinop Oadd (Etempvar _i tint) (Econst_int (Int.repr 1) tint) tint)))
+  (normal_ret_assert
+     (PROP  ()
+      LOCAL  (temp _reset (Vint (Int.repr 1));
+      lvar _ctx_key (Tarray tuchar 64 noattr) (Vptr ckb ckoff);
+      lvar _pad (Tarray tuchar 64 noattr) (Vptr pb pofs);
+      temp _ctx (Vptr cb cofs); temp _key (Vptr kb kofs);
+      temp _len (Vint (Int.repr l)); gvar sha._K256 kv)
+      SEP  ((*`(K_vector kv);*) `(FR);
+      `(data_at Tsh (Tarray tuchar 64 noattr) IPADcont (Vptr pb pofs));
+(*      `(data_at Tsh t_struct_hmac_ctx_st HMS' (Vptr cb cofs));*)
+      `(data_at Tsh (tarray tuchar 64)
+          (map Vint (map Int.repr (HMAC_SHA256.mkKey key))) (Vptr ckb ckoff)) (*;
+      `(data_at Tsh (tarray tuchar (Zlength key))
+          (map Vint (map Int.repr key)) (Vptr kb kofs))*)))).
+Admitted. (*proof ok
+Proof. intros. abbreviate_semax.   
+eapply semax_post'.
+Focus 2.   
+      forward_for_simple_bound' 64 (EX i:Z, 
+        (PROP  ()
+         LOCAL  (temp _reset (Vint (Int.repr 1));
+           lvar _ctx_key (Tarray tuchar 64 noattr) (Vptr ckb ckoff);
+           lvar _pad (Tarray tuchar 64 noattr) (Vptr pb pofs);
+           temp _ctx (Vptr cb cofs); temp _key (Vptr kb kofs);
+           temp _len (Vint (Int.repr l)); gvar sha._K256 kv)
+         SEP  ((*`(K_vector kv);*) `(FR);
+          `(data_at Tsh (Tarray tuchar 64 noattr) 
+             ((sublist 0 i IPADcont) ++ (sublist i 64  (default_val (Tarray tuchar 64 noattr))))
+             (Vptr pb pofs));
+(*          `(data_at Tsh t_struct_hmac_ctx_st (*keyedHMS*)HMS' (Vptr cb cofs));*)
+          `(data_at Tsh (tarray tuchar 64)
+              (map Vint (map Int.repr (HMAC_SHA256.mkKey key))) (Vptr ckb ckoff)) (*;
+         `(data_at Tsh (tarray tuchar (Zlength key)) (map Vint (map Int.repr key))
+              (Vptr kb kofs))*)))).
+      { (*precondition implies "invariant"*)
+        rewrite sublist_nil, sublist_same; trivial. simpl app.
+        entailer.  
+      }
+      { rename H into I. 
+        assert (Xb: exists qb, nth (Z.to_nat i) (HMAC_SHA256.mkKey key) Z0 = qb /\ isbyteZ qb).
+          { destruct (nth_mapIn (Z.to_nat i) (HMAC_SHA256.mkKey key) 0) as [? [? ?]].
+             rewrite mkKey_length.
+              split. apply (Z2Nat.inj_le 0); omega. apply (Z2Nat.inj_lt _ 64); omega.
+            exists x; split; trivial. eapply Forall_forall. apply isbyteZ_mkKey. eassumption. eassumption.
+          }
+        destruct Xb as [qb [Qb isbyteZQb]].
+        assert (X: Znth i (map Vint (map Int.repr (HMAC_SHA256.mkKey key))) Vundef
+                   = Vint (Int.repr qb)). (* (Int.zero_ext 8 q)).*)
+          { unfold Znth. destruct (zlt i 0). omega.
+            rewrite nth_indep with (d':=Vint (Int.repr 0)).
+              Focus 2. repeat rewrite map_length. rewrite mkKey_length. unfold SHA256.BlockSize; simpl. apply (Z2Nat.inj_lt _ 64); omega. 
+            repeat rewrite map_nth. rewrite Qb. trivial. 
+          }
+        forward. entailer.
+
+        apply prop_right. rewrite X. simpl. rewrite <- isbyte_zeroExt8'; trivial.
+               apply (isbyteZ_range _ isbyteZQb). 
+        rewrite X.
+        forward. 
+        unfold Int.xor. 
+        rewrite Int.unsigned_repr. 2: rewrite int_max_unsigned_eq; omega.
+        (*rewrite Int.unsigned_repr. 2: destruct isbyteZQb; rewrite int_max_unsigned_eq; omega.*)
+        exploit (isbyteZ_xor 54 qb); trivial. split; omega.
+        intros isbyteXOR.
+        rewrite <- (isbyte_zeroExt8 qb); trivial.
+        rewrite Int.unsigned_repr. 2: destruct isbyteZQb; rewrite int_max_unsigned_eq; omega.
+        rewrite Z.lxor_comm. remember (Vint (Int.repr (Z.lxor qb 54))) as xorval.
+        forward. entailer. cancel.
+        rewrite field_at_data_at. 
+        apply derives_refl'. f_equal.
+          admit. (*rewrite Z.lxor_comm in isbyteXOR.
+             rewrite UPD_IPAD; try assumption. cancel.*)
+          unfold field_address; simpl. rewrite if_true, Int.add_zero; trivial.
+      }
+Unfocus.
+cbv beta. rewrite sublist_same, sublist_nil, app_nil_r; trivial. entailer.
+subst IPADcont; do 2 rewrite Zlength_map. 
+unfold HMAC_SHA256.mkArgZ in ZLI; rewrite ZLI; trivial.
+Qed. 
+*)
+
+Definition FRAME1 cb cofs ckb ckoff kb kofs key (HMS': reptype t_struct_hmac_ctx_st) := 
+    (field_at Tsh t_struct_hmac_ctx_st [StructField 13%positive] (fst HMS')
+        (Vptr cb cofs)) *
+    (field_at Tsh t_struct_hmac_ctx_st [StructField 15%positive]
+         (snd (snd HMS')) (Vptr cb cofs)) *
+    (data_at Tsh (tarray tuchar 64)
+          (map Vint (map Int.repr (HMAC_SHA256.mkKey key))) (Vptr ckb ckoff)) *
+    (data_at Tsh (tarray tuchar (Zlength key)) (map Vint (map Int.repr key))
+        (Vptr kb kofs)).
+Definition FRAME2 kb kofs cb cofs kv key ipadSHAabs 
+                (HMS' : reptype t_struct_hmac_ctx_st) := (K_vector kv) * 
+   (sha256state_ ipadSHAabs (Vptr cb (Int.add cofs (Int.repr 108)))) *
+   (field_at Tsh t_struct_hmac_ctx_st [StructField 13%positive] (fst HMS')
+       (Vptr cb cofs)) *
+   (field_at Tsh t_struct_hmac_ctx_st [StructField 15%positive]
+       (snd (snd HMS')) (Vptr cb cofs)) * 
+   ( data_at Tsh (tarray tuchar (Zlength key)) (map Vint (map Int.repr key))
+       (Vptr kb kofs)). 
+
+Opaque FRAME1. Opaque FRAME2.
+
+Lemma opadloop Espec pb pofs cb cofs ckb ckoff kb kofs l key kv 
+(HMS' : reptype t_struct_hmac_ctx_st): forall
+(KL1 : l = Zlength key)
+(KL2 : 0 <= l <= Int.max_signed)
+(KL3 : l * 8 < two_p 64)
+(KHMS : HMS' = HMS)
+(h1 : hmacabs)
+(IPADcont : list val)
+(HeqIPADcont : IPADcont =
+              map Vint
+                (map Int.repr
+                   (map Byte.unsigned
+                      (HMAC_SHA256.mkArg
+                         (map Byte.repr (HMAC_SHA256.mkKey key)) Ipad))))
+(OPADcont : list val)
+(HeqOPADcont : OPADcont =
+              map Vint
+                (map Int.repr
+                   (map Byte.unsigned
+                      (HMAC_SHA256.mkArg
+                         (map Byte.repr (HMAC_SHA256.mkKey key)) Opad))))
+(ZLI : Zlength
+        (HMAC_SHA256.mkArgZ (map Byte.repr (HMAC_SHA256.mkKey key)) Ipad) = 64)
+(ZLO : Zlength
+        (HMAC_SHA256.mkArgZ (map Byte.repr (HMAC_SHA256.mkKey key)) Opad) = 64)
+(isbyte_key : Forall isbyteZ key)
+(FC_C : field_compatible t_struct_hmac_ctx_st [] (Vptr cb cofs))
+(VF_HMS' : value_fits true t_struct_hmac_ctx_st HMS')
+(FC_ICTX : field_compatible t_struct_hmac_ctx_st [StructField 14%positive]
+            (Vptr cb cofs))
+(*Delta := abbreviate : tycontext*)
+(ipadSHAabs : s256abs)
+(ipadAbs_def : update_abs
+                (HMAC_SHA256.mkArgZ (map Byte.repr (HMAC_SHA256.mkKey key))
+                   Ipad) init_s256abs ipadSHAabs),
+@semax CompSpecs Espec
+  (initialized_list [_reset; _i] (func_tycontext f_HMAC_Init HmacVarSpecs HmacFunSpecs))
+  (PROP  ()
+   LOCAL  (temp _reset (Vint (Int.repr 1));
+   lvar _ctx_key (Tarray tuchar 64 noattr) (Vptr ckb ckoff);
+   lvar _pad (Tarray tuchar 64 noattr) (Vptr pb pofs);
+   temp _ctx (Vptr cb cofs); temp _key (Vptr kb kofs);
+   temp _len (Vint (Int.repr l)); gvar sha._K256 kv)
+   SEP  (`(K_vector kv);
+   `(sha256state_ ipadSHAabs (Vptr cb (Int.add cofs (Int.repr 108))));
+   `(data_block Tsh
+       (HMAC_SHA256.mkArgZ (map Byte.repr (HMAC_SHA256.mkKey key)) Ipad)
+       (Vptr pb pofs)); `(FRAME1 cb cofs ckb ckoff kb kofs key HMS')))
+  (Sfor (Sset _i (Econst_int (Int.repr 0) tint))
+     (Ebinop Olt (Etempvar _i tint) (Econst_int (Int.repr 64) tint) tint)
+     (Ssequence
+        (Sset _aux
+           (Ecast
+              (Ederef
+                 (Ebinop Oadd (Evar _ctx_key (tarray tuchar 64))
+                    (Etempvar _i tint) (tptr tuchar)) tuchar) tuchar))
+        (Sassign
+           (Ederef
+              (Ebinop Oadd (Evar _pad (tarray tuchar 64)) (Etempvar _i tint)
+                 (tptr tuchar)) tuchar)
+           (Ebinop Oxor (Econst_int (Int.repr 92) tint)
+              (Etempvar _aux tuchar) tint)))
+     (Sset _i
+        (Ebinop Oadd (Etempvar _i tint) (Econst_int (Int.repr 1) tint) tint)))
+  (normal_ret_assert 
+     (PROP ()
+      LOCAL (temp _reset (Vint (Int.repr 1));
+             lvar _ctx_key (Tarray tuchar 64 noattr) (Vptr ckb ckoff);
+             lvar _pad (Tarray tuchar 64 noattr) (Vptr pb pofs); temp _ctx (Vptr cb cofs);
+             temp _key (Vptr kb kofs); temp _len (Vint (Int.repr l)); gvar sha._K256 kv)
+      SEP  (`(K_vector kv);
+            `(sha256state_ ipadSHAabs (Vptr cb (Int.add cofs (Int.repr 108))));
+            `(data_at Tsh (Tarray tuchar 64 noattr) OPADcont (Vptr pb pofs));
+            `(FRAME1 cb cofs ckb ckoff kb kofs key HMS')))).
+Proof. intros. abbreviate_semax. 
+eapply semax_post'.
+Focus 2.   
+      forward_for_simple_bound' 64 (EX i:Z, 
+        (PROP  ()
+         LOCAL  (temp _reset (Vint (Int.repr 1));
+            lvar _ctx_key (Tarray tuchar 64 noattr) (Vptr ckb ckoff);
+            lvar _pad (Tarray tuchar 64 noattr) (Vptr pb pofs);
+            temp _ctx (Vptr cb cofs); temp _key (Vptr kb kofs);
+            temp _len (Vint (Int.repr l)); gvar sha._K256 kv)
+         SEP  (`(K_vector kv); `(sha256state_ ipadSHAabs (Vptr cb (Int.add cofs (Int.repr 108))));
+          `(data_at Tsh (Tarray tuchar 64 noattr) 
+              ((sublist 0 i OPADcont) ++ (sublist i 64 IPADcont)) (Vptr pb pofs));
+          `(FRAME1 cb cofs ckb ckoff kb kofs key HMS')))).
+      { (*precondition implies "invariant"*)
+        unfold data_block.
+        rewrite sublist_nil, sublist_same; trivial.
+          simpl app. entailer. cancel. rewrite ZLI. unfold tarray, HMAC_SHA256.mkArgZ. trivial.
+        subst IPADcont. do 2 rewrite Zlength_map. unfold HMAC_SHA256.mkArgZ in ZLI; rewrite ZLI. trivial. 
+      } 
+      { rename H into I. 
+        assert (Xb: exists qb, nth (Z.to_nat i) (HMAC_SHA256.mkKey key) Z0 = qb /\ isbyteZ qb).
+          { destruct (nth_mapIn (Z.to_nat i) (HMAC_SHA256.mkKey key) 0) as [? [? ?]].
+             rewrite mkKey_length.
+              split. apply (Z2Nat.inj_le 0); omega. apply (Z2Nat.inj_lt _ 64); omega.
+            exists x; split; trivial. eapply Forall_forall. apply isbyteZ_mkKey. eassumption. eassumption.
+          }
+        destruct Xb as [qb [Qb isbyteZQb]].
+        assert (X: Znth i (map Vint (map Int.repr (HMAC_SHA256.mkKey key))) Vundef
+                   = Vint (Int.repr qb)). (* (Int.zero_ext 8 q)).*)
+          { unfold Znth. destruct (zlt i 0). omega.
+            rewrite nth_indep with (d':=Vint (Int.repr 0)).
+              Focus 2. repeat rewrite map_length. rewrite mkKey_length. unfold SHA256.BlockSize; simpl. apply (Z2Nat.inj_lt _ 64); omega. 
+            repeat rewrite map_nth. rewrite Qb. trivial. 
+          }
+
+        gather_SEP 0 1 2 3. 
+        replace_SEP 0 (`(FRAME2 kb kofs cb cofs kv key ipadSHAabs HMS') *
+                       `(data_at Tsh (Tarray tuchar 64 noattr)
+                           (sublist 0 i OPADcont ++ sublist i 64 IPADcont) (Vptr pb pofs)) *
+                       `(data_at Tsh (tarray tuchar 64)
+                           (map Vint (map Int.repr (HMAC_SHA256.mkKey key))) (Vptr ckb ckoff))).
+        { entailer. Transparent FRAME1. Transparent FRAME2. Transparent default_val.
+            unfold FRAME1, FRAME2, HMS, default_val. simpl. cancel.
+        } Opaque FRAME1. Opaque FRAME2. 
+        normalize.
+        forward. Opaque default_val. (*Issue : forward succeeds in 3secs, but if 
+              we put the Opaque declaration before the forword (next to Opaqye FRAME2, as one would expect),
+              the forward leads to memory exhaustion. *)
+        { entailer.
+          apply prop_right. rewrite X. simpl. rewrite <- isbyte_zeroExt8'; trivial.
+                apply (isbyteZ_range _ isbyteZQb). 
+        }
+        rewrite X.
+        forward.
+        entailer. rewrite field_at_data_at. 
+        Transparent FRAME1. Transparent FRAME2. Transparent default_val.
+            unfold FRAME1, FRAME2, HMS, default_val. simpl. cancel.
+        apply derives_refl'. f_equal. admit. (*OPAD*)
+        unfold field_address; simpl. rewrite if_true, Int.add_zero; trivial.
+      }
+Unfocus.
+cbv beta. rewrite sublist_same, sublist_nil, app_nil_r; trivial. admit. 
+subst OPADcont; do 2 rewrite Zlength_map. 
+unfold HMAC_SHA256.mkArgZ in ZLO; rewrite ZLO; trivial.
+Qed. 
+
+Opaque FRAME1. Opaque FRAME2. 
 
 Lemma init_part2: forall
 (Espec : OracleKind)
@@ -280,8 +564,8 @@ Lemma init_part2: forall
 (ctx' : name _ctx)
 (key' : name _key)
 (len' : name _len)
-(Delta := initialized _reset 
-       (func_tycontext f_HMAC_Init HmacVarSpecs HmacFunSpecs))
+(*(Delta := initialized _reset 
+       (func_tycontext f_HMAC_Init HmacVarSpecs HmacFunSpecs))*)
 (cb : block)
 (cofs : int)
 (pad : val)
@@ -306,29 +590,9 @@ Lemma init_part2: forall
           SEP  (`(data_at_ Tsh (tarray tuchar 64) pad);
                 `(data_at_ Tsh (Tarray tuchar 64 noattr) (Vptr ckb ckoff)); 
                 `(initPostResetConditional r (Vptr cb cofs) k h1 key (fst (snd shaStates)) (snd (snd (snd shaStates))));
-                `(K_vector kv)))
-(*WAS:(HeqPostResetBranch : PostResetBranch =
-                     EX  iSA : s256abs,
-                     (EX  iS : s256state,
-                      (EX  oSA : s256abs,
-                       (EX  oS : s256state,
-                        PROP 
-                        (innerShaInit (map Byte.repr (HMAC_SHA256.mkKey key))
-                           iSA /\
-                         s256_relate iSA iS /\
-                         outerShaInit (map Byte.repr (HMAC_SHA256.mkKey key))
-                           oSA /\ s256_relate oSA oS)
-                        LOCAL  (`(eq pad) (eval_var _pad (tarray tuchar 64));
-                        `(eq (Vptr cb cofs)) (eval_id _ctx);
-                        `(eq ctxkey) (eval_var _ctx_key (tarray tuchar 64));
-                        `(eq k) (eval_id _key);
-                        `(eq (Vint (Int.repr l))) (eval_id _len);
-                        `(eq KV) (eval_var sha._K256 (tarray tuint 64)))
-                        SEP  (`(data_at_ Tsh (tarray tuchar 64) pad);
-                        `(data_at_ Tsh (tarray tuchar 64) ctxkey);
-                        `(initPostResetConditional r c k h1 key iS oS);
-                        `(K_vector KV))))))*),
-@semax Espec Delta
+                `(K_vector kv))),
+@semax CompSpecs Espec (*Delta*) (initialized _reset 
+       (func_tycontext f_HMAC_Init HmacVarSpecs HmacFunSpecs))
   (PROP  ()
    LOCAL  (temp _reset (Vint (Int.repr r));
    lvar _ctx_key (tarray tuchar 64) (Vptr ckb ckoff); lvar _pad (tarray tuchar 64) pad;
@@ -442,7 +706,10 @@ Lemma init_part2: forall
             LOCAL ()
             SEP  (`(hmacstate_ h c); `(initPostKey k key); `(K_vector kv))))
         (stackframe_of f_HMAC_Init))).
-Proof. intros.
+Proof. intros. abbreviate_semax.
+    (* Issue: Potential Coq (8.4?) bug about type equalities*)
+    assert (HH: exists HMS': reptype t_struct_hmac_ctx_st, HMS'=HMS). exists HMS; reflexivity.
+    destruct HH as [HMS' KHMS].
 forward_if PostResetBranch. 
   { (* THEN*)
     rename H into r_true. 
@@ -469,22 +736,23 @@ forward_if PostResetBranch.
          SEP  (`(K_vector kv);
                `(data_at Tsh (Tarray tuchar 64 noattr)
                    (default_val (Tarray tuchar 64 noattr)) (Vptr pb pofs));
-               `(data_at Tsh t_struct_hmac_ctx_st keyedHMS (Vptr cb cofs));
+               `(data_at Tsh t_struct_hmac_ctx_st (*keyedHMS*)HMS' (Vptr cb cofs));
                `(data_at Tsh (tarray tuchar 64) (map Vint (map Int.repr (HMAC_SHA256.mkKey key)))
                   (Vptr ckb ckoff));
                `(data_at Tsh (tarray tuchar (Zlength key)) (map Vint (map Int.repr key)) k))).
-    { clear HeqPostResetBranch PostResetBranch.
+    { clear POSTCONDITION HeqPostResetBranch PostResetBranch.
       unfold initPostKeyNullConditional. entailer.
       destruct key'; try contradiction.
       (*integer, ie key==NULL*)
-          simpl in TC0. subst i. simpl. if_tac. subst r. inversion r_true.
+          simpl in TC. subst i. simpl. if_tac. subst r. inversion r_true.
           apply andp_right. entailer. entailer.
       (*key == Vptr*)
        if_tac. subst r. inversion r_true.
           entailer. cancel.
     }
     normalize. destruct R; subst r. omega. clear H. rename H0 into isbyte_key.
-    assert_PROP (isptr k). entailer. apply isptrD in H; destruct H as [kb [kofs HK]]. subst k.
+    assert_PROP (isptr k). entailer. apply isptrD in H; destruct H as [kb [kofs HK]]. 
+    rewrite HK in *. 
 
     eapply semax_seq'. (*TODO: using forward_seq here introduces another Delta0 in goal2 - but it worked fine before I split this off into file XXX_part2.v *)
     instantiate (1:= 
@@ -496,252 +764,152 @@ forward_if PostResetBranch.
       temp _len (Vint (Int.repr l)); gvar sha._K256 kv)
    SEP  (`(K_vector kv);
      `(data_at Tsh (Tarray tuchar 64 noattr) IPADcont (Vptr pb pofs));
-     `(data_at Tsh t_struct_hmac_ctx_st keyedHMS (Vptr cb cofs));
+     `(data_at Tsh t_struct_hmac_ctx_st (*keyedHMS*)HMS' (Vptr cb cofs));
      `(data_at Tsh (tarray tuchar 64)
          (map Vint (map Int.repr (HMAC_SHA256.mkKey key))) (Vptr ckb ckoff));
      `(data_at Tsh (tarray tuchar (Zlength key)) (map Vint (map Int.repr key))
          (Vptr kb kofs))))).
     { (*ipad loop*)
-      forward_for_simple_bound' 64 (EX i:Z, 
-        (PROP  ()
-         LOCAL  (temp _reset (Vint (Int.repr 1));
-           lvar _ctx_key (Tarray tuchar 64 noattr) (Vptr ckb ckoff);
-           lvar _pad (Tarray tuchar 64 noattr) (Vptr pb pofs);
-           temp _ctx (Vptr cb cofs); temp _key (Vptr kb kofs);
-           temp _len (Vint (Int.repr l)); gvar sha._K256 kv)
-         SEP  (`(K_vector kv);
-          `(data_at Tsh (Tarray tuchar 64 noattr) (FIRSTN i IPADcont) (Vptr pb pofs));
-          `(data_at Tsh t_struct_hmac_ctx_st keyedHMS (Vptr cb cofs));
-          `(data_at Tsh (tarray tuchar 64)
-              (map Vint (map Int.repr (HMAC_SHA256.mkKey key))) (Vptr ckb ckoff));
-         `(data_at Tsh (tarray tuchar (Zlength key)) (map Vint (map Int.repr key))
-              (Vptr kb kofs))))).
-      { (*precondition implies "invariant"*)
-        clear HeqPostResetBranch. entailer. 
-      } 
-      { unfold normal_ret_assert. simpl. intros rho. entailer. cancel.
-        rewrite FIRSTN_precise. cancel.
-         do 2 rewrite Zlength_map. apply ZLI. 
-      }
-      { rename H into I. 
-        subst PostResetBranch.
-        assert (Xb: exists qb, nth (Z.to_nat i) (HMAC_SHA256.mkKey key) Z0 = qb /\ isbyteZ qb).
-          { destruct (nth_mapIn (Z.to_nat i) (HMAC_SHA256.mkKey key) 0) as [? [? ?]].
-             rewrite mkKey_length.
-              split. apply (Z2Nat.inj_le 0); omega. apply (Z2Nat.inj_lt _ 64); omega.
-            exists x; split; trivial. eapply Forall_forall. apply isbyteZ_mkKey. eassumption. eassumption.
-          }
-        destruct Xb as [qb [Qb isbyteZQb]].
-        assert (X: Znth i (map Vint (map Int.repr (HMAC_SHA256.mkKey key))) Vundef
-                   = Vint (Int.repr qb)). (* (Int.zero_ext 8 q)).*)
-          { unfold Znth. destruct (zlt i 0). omega.
-            rewrite nth_indep with (d':=Vint (Int.repr 0)).
-              Focus 2. repeat rewrite map_length. rewrite mkKey_length. unfold SHA256.BlockSize; simpl. apply (Z2Nat.inj_lt _ 64); omega. 
-            repeat rewrite map_nth. rewrite Qb. trivial. 
-          }
-        forward. entailer.
-        apply prop_right. rewrite X. simpl. rewrite <- isbyte_zeroExt8'; trivial.
-               apply (isbyteZ_range _ isbyteZQb). 
-        unfold force_val. rewrite sem_cast_i2i_correct_range.
-            Focus 2. apply Znth_map_Vint_is_int_I8.
-                     apply isbyteZ_mkKey. assumption.
-                     rewrite Zlength_correct, mkKey_length. unfold SHA256.BlockSize; simpl; assumption.
-        rewrite X.
-        forward v. subst v.
-        unfold Int.xor. 
-        rewrite Int.unsigned_repr. 2: rewrite int_max_unsigned_eq; omega.
-        rewrite Int.unsigned_repr. 2: destruct isbyteZQb; rewrite int_max_unsigned_eq; omega.
-        exploit (isbyteZ_xor 54 qb); trivial. split; omega.
-        intros isbyteXOR.
-        rewrite <- isbyte_zeroExt8; trivial.
-        rewrite Z.lxor_comm. remember (Vint (Int.repr (Z.lxor qb 54))) as xorval.
-        forward. simpl. intros rho. entailer. cancel.
-        rewrite Z.lxor_comm in isbyteXOR.
-        rewrite UPD_IPAD; try assumption. cancel.
-      }
+      (*semax_subcommand HmacVarSpecs HmacFunSpecs f_HMAC_Init.*)
+      eapply semax_pre_post.
+      Focus 3. eapply (ipad_loop Espec pb pofs cb cofs ckb ckoff kb kofs l key kv HMS' 
+                         (K_vector kv * data_at Tsh t_struct_hmac_ctx_st HMS' (Vptr cb cofs)
+                          * data_at Tsh (tarray tuchar (Zlength key)) (map Vint (map Int.repr key))
+                         (Vptr kb kofs))); eassumption.
+      apply andp_left2. entailer. cancel.
+      intros ? ?. apply andp_left2. apply assert_lemmas.normal_ret_assert_derives'.
+                  entailer. cancel.
     }
 
-    (*continuation after ipad-loop*)   
-    unfold_data_at 2%nat. normalize.
-    rewrite (field_at_data_at Tsh t_struct_hmac_ctx_st [StructField _i_ctx]). 
-    (*extract field-address info before doing anything else*)
-       assert_PROP (isptr (field_address t_struct_hmac_ctx_st [StructField _i_ctx]
-          (Vptr cb cofs))). entailer.
-       apply isptrD in H. destruct H as [cbI [cIoff COffI]]. rewrite COffI in *.
-    unfold field_address in COffI.
-    remember (field_compatible_dec t_struct_hmac_ctx_st [StructField _i_ctx]
-              (Vptr cb cofs)) as s.
-    destruct s; simpl in *; inversion COffI. simpl in *. subst cbI. rewrite COffI. clear COffI. 
+    (*continuation after ipad-loop*) 
+    assert_PROP (field_compatible t_struct_hmac_ctx_st [] (Vptr cb cofs)) as FC_C by entailer.
+    unfold data_at at 2. unfold_field_at 1%nat. normalize.
+    rename H into VF_HMS'.
+
+    gather_SEP 0 2 5 6.
+    replace_SEP 0 (`(FRAME1 cb cofs ckb ckoff kb kofs key HMS')).
+    { subst HMS'. Transparent default_val. Transparent FRAME1. 
+         unfold HMS, FRAME1, default_val. entailer. (*Issue: again unfold default_val here is the key *)
+    }
+Opaque FRAME1. Opaque default_val.
+    rewrite (field_at_data_at  Tsh t_struct_hmac_ctx_st [StructField 14%positive]). (*ie i_ctx*)
+    assert_PROP (field_compatible t_struct_hmac_ctx_st [StructField 14%positive] (Vptr cb cofs)) as FC_ICTX.
+    { apply prop_right. clear - FC_C. red in FC_C; red; intuition. split; trivial. right; left; trivial. }
+    unfold field_address; simpl. rewrite if_true; trivial. unfold field_offset, fieldlist.field_offset2; simpl.
 
     (*Call to _SHA256_Init*)
-    forward_call' (Vptr cb cIoff).
-(*       subst cIoff. 
-       unfold nested_field_offset2; simpl. *)
+    unfold field_type; simpl. 
+    rewrite KHMS at 2. (*Issue: note: don't rewrite in the FRAME1-erm*)
+    Transparent default_val. unfold HMS, default_val; simpl. Opaque default_val.
+    forward_call (Vptr cb (Int.add cofs (Int.repr 108))). 
 
     (*Call to _SHA256_Update*)
-    Opaque firstn. 
-    forward_call' (init_s256abs, 
-            HMAC_SHA256.mkArgZ (map Byte.repr (HMAC_SHA256.mkKey key)) Ipad,
-            Vptr cb cIoff, Vptr pb pofs, Tsh, 64, kv) ipadSHAabs.
-    { assert (FR: Frame = [
-        (field_at Tsh t_struct_hmac_ctx_st [StructField _o_ctx] emptySha (Vptr cb cofs));
-        (field_at Tsh t_struct_hmac_ctx_st [StructField _md_ctx] emptySha (Vptr cb cofs));
-        (data_at Tsh (tarray tuchar 64) (map Vint (map Int.repr (HMAC_SHA256.mkKey key))) (Vptr ckb ckoff));
-        data_at Tsh (tarray tuchar (Zlength key)) (map Vint (map Int.repr key)) (Vptr kb kofs) ]).
+    forward_call (init_s256abs, 
+                  HMAC_SHA256.mkArgZ (map Byte.repr (HMAC_SHA256.mkKey key)) Ipad,
+                  Vptr cb (Int.add cofs (Int.repr 108)), Vptr pb pofs, Tsh, 64, kv)
+               ipadSHAabs.
+    { unfold data_block. rewrite ZLI, HeqIPADcont. unfold HMAC_SHA256.mkArgZ. 
+      (* Issue: entailer.Anomaly: undefined_evars_of_term: evar not found. Please report.*)
+      assert (FR : Frame = [FRAME1 cb cofs ckb ckoff kb kofs key HMS']).
         subst Frame; reflexivity.
       rewrite FR; clear FR Frame. 
-      entailer. cancel.
-      unfold data_block. rewrite ZLI. entailer. 
-      apply andp_right. 
-        simpl. apply prop_right. apply isbyte_map_ByteUnsigned. cancel. 
+      simpl. normalize. apply andp_right. apply prop_right. apply isbyte_map_ByteUnsigned. cancel. 
+    } 
+    { clear Frame HeqPostResetBranch HeqOPADcont; subst IPADcont.
+        rewrite Zlength_mkArgZ. repeat rewrite map_length. rewrite mkKey_length. intuition. 
     }
-      { clear Frame HeqPostResetBranch HeqOPADcont; subst IPADcont.
-        rewrite Zlength_mkArgZ. repeat rewrite map_length. rewrite mkKey_length. 
-        unfold SHA256.BlockSize; simpl. rewrite int_max_unsigned_eq.
-        unfold two_power_pos, shift_pos. simpl. omega.
-      }
     rename H into ipadAbs_def.
     normalize.
-    rewrite firstn_precise in ipadAbs_def.
-    Focus 2. specialize (Zlength_mkArgZ (map Byte.repr (HMAC_SHA256.mkKey key)) Ipad); intros. 
-            apply coqlib3.Zlength_length in H. rewrite H. repeat rewrite map_length. rewrite mkKey_length. reflexivity.
-            repeat rewrite map_length. rewrite mkKey_length. simpl. omega. 
-    Transparent firstn. 
+    rewrite sublist_same in ipadAbs_def; try rewrite ZLI; trivial.
 
     (*essentially the same for opad*)
     eapply semax_seq'. (* TODO: using forward_seq here introduces another Delta0 in goal2 - but 
                           it worked fine before I split this off into file XXX_part2.v *)
-     instantiate (1:= 
-       (PROP  ()
-        LOCAL  (temp _reset (Vint (Int.repr 1));
-          lvar _ctx_key (Tarray tuchar 64 noattr) (Vptr ckb ckoff);
-          lvar _pad (Tarray tuchar 64 noattr) (Vptr pb pofs);
-          temp _ctx (Vptr cb cofs); temp _key (Vptr kb kofs);
-          temp _len (Vint (Int.repr l)); gvar sha._K256 kv)
-        SEP  (`(K_vector kv);
-         `(sha256state_ ipadSHAabs (Vptr cb cIoff));
-         `(data_at Tsh (Tarray tuchar 64 noattr) OPADcont (Vptr pb pofs));
-         `(field_at Tsh t_struct_hmac_ctx_st [StructField _o_ctx] emptySha (Vptr cb cofs));
-         `(field_at Tsh t_struct_hmac_ctx_st [StructField _md_ctx] emptySha (Vptr cb cofs));
-         `(data_at Tsh (tarray tuchar 64)
-            (map Vint (map Int.repr (HMAC_SHA256.mkKey key))) (Vptr ckb ckoff));
-         `(data_at Tsh (tarray tuchar (Zlength key)) (map Vint (map Int.repr key))
-            (Vptr kb kofs))))).
-
-    { (*opad loop*) 
-      forward_for_simple_bound' 64 (EX i:Z, 
-        (PROP  ()
-         LOCAL  (temp _reset (Vint (Int.repr 1));
-            lvar _ctx_key (Tarray tuchar 64 noattr) (Vptr ckb ckoff);
-            lvar _pad (Tarray tuchar 64 noattr) (Vptr pb pofs);
-            temp _ctx (Vptr cb cofs); temp _key (Vptr kb kofs);
-            temp _len (Vint (Int.repr l)); gvar sha._K256 kv)
-         SEP  (`(K_vector kv); `(sha256state_ ipadSHAabs (Vptr cb cIoff));
-          `(data_at Tsh (Tarray tuchar 64 noattr) ((FIRSTN i OPADcont)++(SKIPN i IPADcont)) (Vptr pb pofs));
-         `(data_at Tsh (tarray tuchar 64)
-              (map Vint (map Int.repr (HMAC_SHA256.mkKey key))) (Vptr ckb ckoff));
-         `(field_at Tsh t_struct_hmac_ctx_st [StructField _o_ctx] emptySha (Vptr cb cofs));
-         `(field_at Tsh t_struct_hmac_ctx_st [StructField _md_ctx] emptySha (Vptr cb cofs));
-        `(data_at Tsh (tarray tuchar (Zlength key)) (map Vint (map Int.repr key)) (Vptr kb kofs))))).
-      { (*precondition implies "invariant"*)
-        clear HeqPostResetBranch.
-        unfold data_block. entailer. cancel. 
-        unfold SKIPN; simpl. rewrite ZLI; cancel.            
-      }
-      { unfold normal_ret_assert. simpl. intros rho. entailer. cancel.
-        rewrite FIRSTN_precise.
-         rewrite SKIPn_short. rewrite app_nil_r.
-         cancel.
-         do 2 rewrite Zlength_map. unfold HMAC_SHA256.mkArgZ in ZLI; rewrite ZLI. omega. 
-         do 2 rewrite Zlength_map. unfold HMAC_SHA256.mkArgZ in ZLO; rewrite ZLO; trivial. 
-      }
-      { rename H into I. 
-        assert (Xb: exists qb, nth (Z.to_nat i) (HMAC_SHA256.mkKey key) Z0 = qb /\ isbyteZ qb).
-          { destruct (nth_mapIn (Z.to_nat i) (HMAC_SHA256.mkKey key) 0) as [? [? ?]].
-             rewrite mkKey_length.
-              split. apply (Z2Nat.inj_le 0); omega. apply (Z2Nat.inj_lt _ 64); omega.
-            exists x; split; trivial. eapply Forall_forall. apply isbyteZ_mkKey. eassumption. eassumption.
-          }
-        destruct Xb as [qb [Qb isbyteZQb]].
-        assert (X: Znth i (map Vint (map Int.repr (HMAC_SHA256.mkKey key))) Vundef
-                   = Vint (Int.repr qb)). (* (Int.zero_ext 8 q)).*)
-          { unfold Znth. destruct (zlt i 0). omega.
-            rewrite nth_indep with (d':=Vint (Int.repr 0)).
-              Focus 2. repeat rewrite map_length. rewrite mkKey_length. unfold SHA256.BlockSize; simpl. apply (Z2Nat.inj_lt _ 64); omega. 
-            repeat rewrite map_nth. rewrite Qb. trivial. 
-          }
-        forward.
-        { entailer. 
-          apply prop_right. rewrite X. simpl. rewrite <- isbyte_zeroExt8'; trivial.
-                apply (isbyteZ_range _ isbyteZQb). 
-        }
-        unfold force_val. rewrite sem_cast_i2i_correct_range.
-        Focus 2. apply Znth_map_Vint_is_int_I8.
-                     apply isbyteZ_mkKey. assumption.
-                     rewrite Zlength_correct, mkKey_length. unfold SHA256.BlockSize; simpl; assumption.
-        rewrite X.
-        forward.
-        entailer. cancel. 
-        rewrite UPD_OPAD; try assumption. cancel.
-      }
+    instantiate (1:= PROP  ()
+       LOCAL  (temp _reset (Vint (Int.repr 1));
+               lvar _ctx_key (Tarray tuchar 64 noattr) (Vptr ckb ckoff);
+               lvar _pad (Tarray tuchar 64 noattr) (Vptr pb pofs); temp _ctx (Vptr cb cofs);
+               temp _key (Vptr kb kofs); temp _len (Vint (Int.repr l)); gvar sha._K256 kv)
+       SEP  (`(K_vector kv);
+             `(sha256state_ ipadSHAabs (Vptr cb (Int.add cofs (Int.repr 108))));
+             `(data_at Tsh (Tarray tuchar 64 noattr) OPADcont (Vptr pb pofs));
+             `(FRAME1 cb cofs ckb ckoff kb kofs key HMS'))). 
+    { (*opad loop*)
+      eapply semax_pre_post.
+      Focus 3. eapply (opadloop Espec pb pofs cb cofs ckb ckoff kb kofs l key kv HMS');
+               try eassumption. 
+      apply andp_left2. apply derives_refl.
+      intros ? ?. apply andp_left2. apply derives_refl.
     }
-    (*continuation after opad-loop*)  
-    rewrite (field_at_data_at Tsh t_struct_hmac_ctx_st [StructField _o_ctx]).
-    assert_PROP (isptr (field_address t_struct_hmac_ctx_st [StructField _o_ctx] (Vptr cb cofs))).
-    { entailer. }
-    apply isptrD in H; destruct H as [cbO [cOoff COffO]]. rewrite COffO in *.
-    unfold field_address in COffO.
-    remember (field_compatible_dec t_struct_hmac_ctx_st [StructField _o_ctx]
-              (Vptr cb cofs)) as s.
-    destruct s; simpl in *; inversion COffO; clear COffO. simpl in *. subst cbO cOoff.
-   
-    (*Call to _SHA256_Init*)  
+
+    (*continuation after opad-loop*) 
+    Transparent FRAME1. unfold FRAME1. 
+    rewrite (field_at_data_at Tsh t_struct_hmac_ctx_st [StructField 15%positive]).
+    assert_PROP (field_compatible t_struct_hmac_ctx_st [StructField 15%positive] (Vptr cb cofs)) as FC_OCTX.
+    { apply prop_right. clear - FC_C. red in FC_C; red; intuition. split; trivial. right; right; left; trivial. }
+    unfold field_address; simpl. rewrite if_true; trivial. unfold field_offset, fieldlist.field_offset2; simpl.
+
+    (*Call to _SHA256_Init*)
+    unfold field_type; simpl. Transparent default_val. normalize. Opaque default_val.
+    gather_SEP 0 2 3 5. 
+Definition FRAME3 (kb cb ckb: block) kofs cofs ckoff key ipadSHAabs (HMS' : reptype t_struct_hmac_ctx_st):= 
+       (field_at Tsh t_struct_hmac_ctx_st [StructField 13%positive] (fst HMS') (Vptr cb cofs) ) * 
+       (data_at Tsh (tarray tuchar 64) (map Vint (map Int.repr (HMAC_SHA256.mkKey key))) (Vptr ckb ckoff)) *
+       (data_at Tsh (tarray tuchar (Zlength key)) (map Vint (map Int.repr key)) (Vptr kb kofs)) *
+       (sha256state_ ipadSHAabs (Vptr cb (Int.add cofs (Int.repr 108)))).
+    replace_SEP 0 (`(FRAME3 kb cb ckb kofs cofs ckoff key ipadSHAabs HMS')).
+    { Transparent default_val. rewrite KHMS. entailer!. }  (*Don't use entailer here!!*)
     (*TODO: one of the most recent changes in floyd (or elsewhere?) meant
     that I have to do the following unfold here t get forward_call' to apply*)
-    unfold MORE_COMMANDS, abbreviate. 
-    forward_call' (Vptr cb (Int.add cofs (Int.repr 216))).
-    
+    unfold MORE_COMMANDS, abbreviate.
+    (*This line is crucial: *) rewrite KHMS. unfold HMS; simpl.
+    forward_call (Vptr cb (Int.add cofs (Int.repr 216))).
+ 
     (* Call to sha_update*)
-    (* TODO: investigate the need for the semax_seq_skip. *)
-    rewrite -> semax_seq_skip.
-    Opaque firstn. 
-    forward_call' (init_s256abs, 
+    forward_call (init_s256abs, 
             HMAC_SHA256.mkArgZ (map Byte.repr (HMAC_SHA256.mkKey key)) Opad,
             Vptr cb (Int.add cofs (Int.repr 216)),
             Vptr pb pofs, Tsh, 64, kv)  opadSHAabs.
-    { assert (FR: Frame = [(sha256state_ ipadSHAabs (Vptr cb cIoff));
-         (field_at Tsh t_struct_hmac_ctx_st [StructField _md_ctx] emptySha (Vptr cb cofs));
-         (data_at Tsh (tarray tuchar 64) (map Vint (map Int.repr (HMAC_SHA256.mkKey key))) (Vptr ckb ckoff));
-         (data_at Tsh (tarray tuchar (Zlength key)) (map Vint (map Int.repr key)) (Vptr kb kofs))]).
+    { unfold data_block. rewrite ZLO, HeqOPADcont. 
+      (*Issue: same as in ipad loop: need to instantiate Frame manually:
+           entailer/entailer!/normalize don't appear to terminate, or creash with "anomaly"*)
+      assert (FR : Frame = [FRAME3 kb cb ckb kofs cofs ckoff key ipadSHAabs
+                             (default_val t_struct_hmac_ctx_st)]).
         subst Frame; reflexivity.
       rewrite FR; clear FR Frame. 
-      cancel. unfold data_block. rewrite ZLO.
-      entailer. simpl; normalize.
-      apply andp_right. 
-        simpl. apply prop_right. apply isbyte_map_ByteUnsigned.
-      cancel.
+      simpl. normalize. apply andp_right. apply prop_right. apply isbyte_map_ByteUnsigned. cancel. 
     }
-    { clear Frame HeqPostResetBranch HeqIPADcont; subst OPADcont.
-      rewrite Zlength_mkArgZ. repeat rewrite map_length. rewrite mkKey_length. 
-      unfold SHA256.BlockSize; simpl. rewrite int_max_unsigned_eq.
-      unfold two_power_pos, shift_pos. simpl. omega.
-    } 
+    { rewrite ZLO. intuition. } 
+
     rename H into opadAbs_def.
     normalize.
-    rewrite firstn_precise in opadAbs_def.
-    Focus 2. specialize (Zlength_mkArgZ (map Byte.repr (HMAC_SHA256.mkKey key)) Opad); intros. 
-            apply coqlib3.Zlength_length in H. rewrite H. repeat rewrite map_length. rewrite mkKey_length. reflexivity.
-            repeat rewrite map_length. rewrite mkKey_length. simpl. omega. 
-    Transparent firstn. 
+    rewrite sublist_same in opadAbs_def; try rewrite ZLO; trivial.
 
-    subst PostResetBranch; entailer. unfold sha256state_; normalize. rename r into iUpd. rename x into oUpd.
-        apply (exp_right (ipadSHAabs,(iUpd,(opadSHAabs,oUpd)))). entailer.
-        unfold data_block, initPostResetConditional. simpl.
-        rewrite ZLO. entailer. cancel.
-        unfold_data_at 3%nat. cancel.
+    subst PostResetBranch; entailer.
+    unfold FRAME3, sha256state_, default_val; simpl.
+    normalize. rename r into iUpd. rename x into oUpd.
+    Exists (ipadSHAabs,(iUpd,(opadSHAabs,oUpd))). simpl.
+    apply andp_right. apply prop_right. intuition.
+    apply andp_right. apply prop_right. intuition.
+    cancel.
+        unfold data_block. (* initPostResetConditional. simpl.*)
+        rewrite ZLO. normalize. cancel.
+
+        (*Issue: VST's canceler fails to cancel the pad terms (Vptr pb pofs), 
+            since they';re at different CompSpecs*)
+        repeat rewrite <- sepcon_assoc.
+        repeat rewrite sepcon_assoc. rewrite sepcon_comm. repeat rewrite <- sepcon_assoc.
+        repeat rewrite sepcon_assoc. 
+        apply sepcon_derives. eapply derives_trans. apply data_at_data_at_. apply derives_refl.
+
+    unfold data_at at 3. unfold_field_at 2%nat. 
     rewrite (field_at_data_at Tsh t_struct_hmac_ctx_st [StructField _i_ctx]).
     rewrite (field_at_data_at Tsh t_struct_hmac_ctx_st [StructField _o_ctx]).
-    unfold field_address. rewrite <- Heqs, <- Heqs0. simpl. cancel.
+    unfold field_address. rewrite if_true; trivial. rewrite if_true; trivial.
+       unfold nested_field_type2, nested_field_offset2; simpl.
+       unfold field_type, field_offset, fieldlist.field_offset2; simpl.
+     apply andp_right. apply prop_right. unfold postResetHMS. admit. (*TODO: VlaueFits*)
+     cancel.
   }
   { (*ELSE*) 
     forward. subst. unfold initPostKeyNullConditional. entailer. 
@@ -749,11 +917,18 @@ forward_if PostResetBranch.
     simpl; clear H. destruct key'; try solve[entailer]. 
     unfold hmacstate_PreInitNull, hmac_relate_PreInitNull; simpl.
     destruct h1; entailer.
-    destruct (Int.eq i Int.zero); entailer.
-    apply (exp_right (iSha, (iCtx v, (oSha, oCtx v)))).
-    entailer. cancel.
+    if_tac. Focus 2. entailer. 
+    normalize.
+    Exists (iSha, (iCtx v, (oSha, oCtx v))). simpl. 
+    apply andp_right. apply prop_right. intuition.
+    apply andp_right. apply prop_right. intuition.
+    cancel.
     unfold hmacstate_PreInitNull, hmac_relate_PreInitNull; simpl.
-    apply (exp_right v). apply (exp_right x).
-    entailer.
-   } 
+    Exists v x.
+    apply andp_right. apply prop_right. intuition.
+    cancel.
+   }
+intros ? ?. apply andp_left2.  
+   unfold POSTCONDITION, abbreviate. rewrite overridePost_overridePost. 
+   apply derives_refl. 
 Qed.
